<?xml version="1.0"?>
<rdf:RDF xmlns="http://vocab.linkeddata.es/datosabiertos/def/transporte/censovehiculos#"
     xml:base="http://vocab.linkeddata.es/datosabiertos/def/transporte/censovehiculos"
     xmlns:mod="https://w3id.org/mod#"
     xmlns:owl="http://www.w3.org/2002/07/owl#"
     xmlns:rdf="http://www.w3.org/1999/02/22-rdf-syntax-ns#"
     xmlns:xml="http://www.w3.org/XML/1998/namespace"
     xmlns:xsd="http://www.w3.org/2001/XMLSchema#"
     xmlns:rdfs="http://www.w3.org/2000/01/rdf-schema#"
     xmlns:vann="http://purl.org/vocab/vann/"
     xmlns:terms="http://purl.org/dc/terms/">
    <owl:Ontology rdf:about="http://vocab.linkeddata.es/datosabiertos/def/transporte/censovehiculos">
        <owl:versionIRI rdf:resource="http://vocab.linkeddata.es/datosabiertos/def/transporte/censovehiculos/0.1.0"/>
        <terms:created rdf:datatype="http://www.w3.org/2001/XMLSchema#date">2026-01-29</terms:created>
        <terms:creator xml:lang="es">Daniel Doña</terms:creator>
        <terms:creator>Edna Ruckhaus</terms:creator>
        <terms:creator>Lucía Sánchez</terms:creator>
        <terms:creator>Oscar Corcho</terms:creator>
        <terms:description xml:lang="es">El propósito de esta ontología es el de proporcionar un vocabulario común para la representación de las entidades y datos principales del censo o registro de vehículos. Su alcance se limita a los datos que pueden ser utilizados con los propósitos de cobro de impuestos por parte de las entidades locales o de gestión de la movilidad (permisos de aparcamiento, permisos de acceso a zonas específicas, etc.), que son parte de las funciones habituales de las entidades locales. Quedan fuera del alcance de la ontología otros aspectos relacionados con los vehículos, como pueden ser los datos de sus permisos de circulación, inspecciones técnicas, etc., que podrían ser objeto de una extensión de esta ontología o de su evolución en el futuro, si se considera relevante.</terms:description>
        <terms:description xml:lang="en">The purpose of this ontology is to provide a common vocabulary for representing the main entities and data of the vehicle census or registry. Its scope is limited to the data that may be used for purposes such as tax collection by local authorities or mobility management (parking permits, access permits to specific zones, etc.), which are part of the usual functions of local entities. Other aspects related to vehicles, such as data concerning driving permits, technical inspections, and similar information, are outside the scope of this ontology. These could be addressed through an extension of this ontology or through its future evolution, if considered relevant.</terms:description>
        <terms:hasFormat>http://vocab.linkeddata.es/datosabiertos/def/transporte/censovehiculos.owl</terms:hasFormat>
        <terms:license rdf:resource="https://creativecommons.org/licenses/by/4.0/"/>
        <vann:preferredNamespacePrefix>edintveh</vann:preferredNamespacePrefix>
        <vann:preferredNamespaceUri rdf:resource="http://vocab.linkeddata.es/datosabiertos/def/transporte/censovehiculos#"/>
        <owl:versionInfo>0.1.0</owl:versionInfo>
    </owl:Ontology>
    


    <!-- 
    ///////////////////////////////////////////////////////////////////////////////////////
    //
    // Annotation properties
    //
    ///////////////////////////////////////////////////////////////////////////////////////
     -->


    


    <!-- http://purl.org/dc/terms/contributor -->


    <owl:AnnotationProperty rdf:about="http://purl.org/dc/terms/contributor"/>
    


    <!-- http://purl.org/dc/terms/created -->


    <owl:AnnotationProperty rdf:about="http://purl.org/dc/terms/created"/>
    


    <!-- http://purl.org/dc/terms/creator -->


    <owl:AnnotationProperty rdf:about="http://purl.org/dc/terms/creator"/>
    


    <!-- http://purl.org/dc/terms/description -->


    <owl:AnnotationProperty rdf:about="http://purl.org/dc/terms/description"/>
    


    <!-- http://purl.org/dc/terms/hasFormat -->


    <owl:AnnotationProperty rdf:about="http://purl.org/dc/terms/hasFormat"/>
    


    <!-- http://purl.org/dc/terms/license -->


    <owl:AnnotationProperty rdf:about="http://purl.org/dc/terms/license"/>
    


    <!-- http://purl.org/dc/terms/title -->


    <owl:AnnotationProperty rdf:about="http://purl.org/dc/terms/title"/>
    


    <!-- http://purl.org/vocab/vann/preferredNamespacePrefix -->


    <owl:AnnotationProperty rdf:about="http://purl.org/vocab/vann/preferredNamespacePrefix"/>
    


    <!-- http://purl.org/vocab/vann/preferredNamespaceUri -->


    <owl:AnnotationProperty rdf:about="http://purl.org/vocab/vann/preferredNamespaceUri"/>
    


    <!-- http://www.w3.org/2002/07/owl#versionIRI -->


    <owl:AnnotationProperty rdf:about="http://www.w3.org/2002/07/owl#versionIRI"/>
    


    <!-- http://www.w3.org/2002/07/owl#versionInfo -->


    <owl:AnnotationProperty rdf:about="http://www.w3.org/2002/07/owl#versionInfo"/>
    


    <!-- https://w3id.org/mod#createdWith -->


    <owl:AnnotationProperty rdf:about="https://w3id.org/mod#createdWith"/>
    


    <!-- 
    ///////////////////////////////////////////////////////////////////////////////////////
    //
    // Datatypes
    //
    ///////////////////////////////////////////////////////////////////////////////////////
     -->


    


    <!-- http://www.w3.org/2001/XMLSchema#date -->


    <rdfs:Datatype rdf:about="http://www.w3.org/2001/XMLSchema#date"/>
    


    <!-- 
    ///////////////////////////////////////////////////////////////////////////////////////
    //
    // Object Properties
    //
    ///////////////////////////////////////////////////////////////////////////////////////
     -->


    


    <!-- http://vocab.ciudadesabiertas.es/def/transporte/trafico#via -->


    <owl:ObjectProperty rdf:about="http://vocab.ciudadesabiertas.es/def/transporte/trafico#via">
        <rdfs:range rdf:resource="http://vocab.ciudadesabiertas.es/def/transporte/trafico#Tramo"/>
    </owl:ObjectProperty>
    


    <!-- http://vocab.linkeddata.es/datosabiertos/def/transporte/censovehiculos#authorisesInSegment -->


    <owl:ObjectProperty rdf:about="http://vocab.linkeddata.es/datosabiertos/def/transporte/censovehiculos#authorisesInSegment">
        <rdfs:domain rdf:resource="http://vocab.linkeddata.es/datosabiertos/def/transporte/censovehiculos#Permit"/>
        <rdfs:range rdf:resource="http://vocab.ciudadesabiertas.es/def/transporte/trafico#Tramo"/>
        <rdfs:comment xml:lang="es">Identifica el segmento de vía para el cual la autorización da permiso para pasar o aparcar</rdfs:comment>
        <rdfs:comment xml:lang="en">It identifies a segment where the permit authorises the vehicle to go through or park</rdfs:comment>
        <rdfs:comment xml:lang="en">authorises in segment</rdfs:comment>
        <rdfs:label xml:lang="es">autoriza en tramo</rdfs:label>
    </owl:ObjectProperty>
    


    <!-- http://vocab.linkeddata.es/datosabiertos/def/transporte/censovehiculos#authorisesInZone -->


    <owl:ObjectProperty rdf:about="http://vocab.linkeddata.es/datosabiertos/def/transporte/censovehiculos#authorisesInZone">
        <rdfs:domain rdf:resource="http://vocab.linkeddata.es/datosabiertos/def/transporte/censovehiculos#Permit"/>
        <rdfs:range rdf:resource="http://vocab.linkeddata.es/datosabiertos/def/commons/zone#TrafficControlledZone"/>
        <rdfs:comment xml:lang="es">Identifica una zona de tráfico regulado para la cual la autorización da permiso para pasar o aparcar</rdfs:comment>
        <rdfs:comment xml:lang="en">It identifies a traffic-controlled zone where the permit authorises the vehicle to go through or park</rdfs:comment>
        <rdfs:comment xml:lang="en">authorises in zone</rdfs:comment>
        <rdfs:label xml:lang="es">autoriza en zona</rdfs:label>
    </owl:ObjectProperty>
    


    <!-- http://vocab.linkeddata.es/datosabiertos/def/transporte/censovehiculos#authorisesVehicle -->


    <owl:ObjectProperty rdf:about="http://vocab.linkeddata.es/datosabiertos/def/transporte/censovehiculos#authorisesVehicle">
        <rdfs:domain rdf:resource="http://vocab.linkeddata.es/datosabiertos/def/transporte/censovehiculos#Permit"/>
        <rdfs:range rdf:resource="http://vocab.linkeddata.es/datosabiertos/def/transporte/censovehiculos#Vehicle"/>
        <rdfs:comment xml:lang="es">Identifica el vehículo al que se refiere la autorización</rdfs:comment>
        <rdfs:comment xml:lang="en">It identifies the vehicle for which the permit is issued</rdfs:comment>
        <rdfs:label xml:lang="en">authorises vehicle</rdfs:label>
        <rdfs:label xml:lang="es">autoriza vehículo</rdfs:label>
    </owl:ObjectProperty>
    


    <!-- http://vocab.linkeddata.es/datosabiertos/def/transporte/censovehiculos#environmentalBadge -->


    <owl:ObjectProperty rdf:about="http://vocab.linkeddata.es/datosabiertos/def/transporte/censovehiculos#environmentalBadge">
        <rdfs:domain rdf:resource="http://vocab.linkeddata.es/datosabiertos/def/transporte/censovehiculos#Vehicle"/>
        <rdfs:range>
            <owl:Class>
                <owl:intersectionOf rdf:parseType="Collection">
                    <rdf:Description rdf:about="http://www.w3.org/2004/02/skos/core#Concept"/>
                    <owl:Restriction>
                        <owl:onProperty rdf:resource="http://www.w3.org/2004/02/skos/core#inScheme"/>
                        <owl:hasValue rdf:resource="http://vocab.linkeddata.es/datosabiertos/kos/edint/VehicleEnvironmentalBadge"/>
                    </owl:Restriction>
                </owl:intersectionOf>
            </owl:Class>
        </rdfs:range>
        <rdfs:comment xml:lang="es">Distintivo ambiental asignado a un vehículo. Los valores son conceptos SKOS que pertenecen a una lista controlada de tipos de autorización (por ejemplo, ECO, B, C, etc.)</rdfs:comment>
        <rdfs:comment xml:lang="en">Environmental badge assigned to a vehicle. The range is a SKOS concept that belongs to a controlled list of permit types (e.g., ECO, B, C, etc.).</rdfs:comment>
        <rdfs:label xml:lang="es">distintivo ambiental del vehículo</rdfs:label>
        <rdfs:label xml:lang="en">environmental badge</rdfs:label>
    </owl:ObjectProperty>
    


    <!-- http://vocab.linkeddata.es/datosabiertos/def/transporte/censovehiculos#permitOwner -->


    <owl:ObjectProperty rdf:about="http://vocab.linkeddata.es/datosabiertos/def/transporte/censovehiculos#permitOwner">
        <rdfs:domain rdf:resource="http://vocab.linkeddata.es/datosabiertos/def/transporte/censovehiculos#Permit"/>
        <rdfs:range rdf:resource="http://vocab.linkeddata.es/datosabiertos/def/transporte/censovehiculos#Owner"/>
        <rdfs:comment xml:lang="es">Identifica al titular (persona u organización) para el cual la autorización está expedida</rdfs:comment>
        <rdfs:comment xml:lang="en">It identifies the person or organisation for which the permit has been issued</rdfs:comment>
        <rdfs:comment xml:lang="en">permit owner</rdfs:comment>
        <rdfs:label xml:lang="es">titular autorización</rdfs:label>
    </owl:ObjectProperty>
    


    <!-- http://vocab.linkeddata.es/datosabiertos/def/transporte/censovehiculos#permitPeriodicity -->


    <owl:ObjectProperty rdf:about="http://vocab.linkeddata.es/datosabiertos/def/transporte/censovehiculos#permitPeriodicity">
        <rdfs:domain rdf:resource="http://vocab.linkeddata.es/datosabiertos/def/transporte/censovehiculos#Permit"/>
        <rdfs:range>
            <owl:Class>
                <owl:intersectionOf rdf:parseType="Collection">
                    <rdf:Description rdf:about="http://www.w3.org/2004/02/skos/core#Concept"/>
                    <owl:Restriction>
                        <owl:onProperty rdf:resource="http://www.w3.org/2004/02/skos/core#inScheme"/>
                        <owl:hasValue rdf:resource="http://vocab.linkeddata.es/datosabiertos/kos/edint/VehiclePermitPeriodicity"/>
                    </owl:Restriction>
                </owl:intersectionOf>
            </owl:Class>
        </rdfs:range>
        <rdfs:comment xml:lang="es">Identifica la periodicidad de la autorización para un vehículo. Los valores son conceptos SKOS que pertenecen a una lista controlada de tipos de autorización (por ejemplo, mensual, anual, etc.)</rdfs:comment>
        <rdfs:comment xml:lang="en">It identifies the periodicity of a vehicle permit. The range is a SKOS concept that belongs to a controlled list of permit types (e.g., monhtly, annual, etc.).</rdfs:comment>
        <rdfs:label xml:lang="es">periodicidad de la autorización</rdfs:label>
        <rdfs:label xml:lang="en">permit periodicity</rdfs:label>
    </owl:ObjectProperty>
    


    <!-- http://vocab.linkeddata.es/datosabiertos/def/transporte/censovehiculos#permitStatus -->


    <owl:ObjectProperty rdf:about="http://vocab.linkeddata.es/datosabiertos/def/transporte/censovehiculos#permitStatus">
        <rdfs:domain rdf:resource="http://vocab.linkeddata.es/datosabiertos/def/transporte/censovehiculos#Permit"/>
        <rdfs:range>
            <owl:Class>
                <owl:intersectionOf rdf:parseType="Collection">
                    <rdf:Description rdf:about="http://www.w3.org/2004/02/skos/core#Concept"/>
                    <owl:Restriction>
                        <owl:onProperty rdf:resource="http://www.w3.org/2004/02/skos/core#inScheme"/>
                        <owl:hasValue rdf:resource="http://vocab.linkeddata.es/datosabiertos/kos/edint/VehiclePermitStatus"/>
                    </owl:Restriction>
                </owl:intersectionOf>
            </owl:Class>
        </rdfs:range>
        <rdfs:comment xml:lang="es">Identifica el estado de la autorización para un vehículo. Los valores son conceptos SKOS que pertenecen a una lista controlada de tipos de autorización (por ejemplo, activo, inactivo, rechazado, etc.)</rdfs:comment>
        <rdfs:comment xml:lang="en">It identifies the status of a vehicle permit. The range is a SKOS concept that belongs to a controlled list of permit types (e.g., active, inactive, rejected, etc.).</rdfs:comment>
        <rdfs:label xml:lang="es">estado de autorización</rdfs:label>
        <rdfs:label xml:lang="en">permit status</rdfs:label>
    </owl:ObjectProperty>
    


    <!-- http://vocab.linkeddata.es/datosabiertos/def/transporte/censovehiculos#permitType -->


    <owl:ObjectProperty rdf:about="http://vocab.linkeddata.es/datosabiertos/def/transporte/censovehiculos#permitType">
        <rdfs:domain rdf:resource="http://vocab.linkeddata.es/datosabiertos/def/transporte/censovehiculos#Permit"/>
        <rdfs:range>
            <owl:Class>
                <owl:intersectionOf rdf:parseType="Collection">
                    <rdf:Description rdf:about="http://www.w3.org/2004/02/skos/core#Concept"/>
                    <owl:Restriction>
                        <owl:onProperty rdf:resource="http://www.w3.org/2004/02/skos/core#inScheme"/>
                        <owl:hasValue rdf:resource="http://vocab.linkeddata.es/datosabiertos/kos/edint/VehiclePermitType"/>
                    </owl:Restriction>
                </owl:intersectionOf>
            </owl:Class>
        </rdfs:range>
        <rdfs:comment xml:lang="es">Identifica el tipo de autorización para un vehículo. Los valores son conceptos SKOS que pertenecen a una lista controlada de tipos de autorización.</rdfs:comment>
        <rdfs:comment xml:lang="en">It identifies the type of vehicle permit. The range is a SKOS concept that belongs to a controlled list of permit types.</rdfs:comment>
        <rdfs:label xml:lang="en">permit type</rdfs:label>
        <rdfs:label xml:lang="es">tipo de autorizacion</rdfs:label>
    </owl:ObjectProperty>
    


    <!-- http://vocab.linkeddata.es/datosabiertos/def/transporte/censovehiculos#propulsionType -->


    <owl:ObjectProperty rdf:about="http://vocab.linkeddata.es/datosabiertos/def/transporte/censovehiculos#propulsionType">
        <rdfs:domain rdf:resource="http://vocab.linkeddata.es/datosabiertos/def/transporte/censovehiculos#Vehicle"/>
        <rdfs:range>
            <owl:Class>
                <owl:intersectionOf rdf:parseType="Collection">
                    <rdf:Description rdf:about="http://www.w3.org/2004/02/skos/core#Concept"/>
                    <owl:Restriction>
                        <owl:onProperty rdf:resource="http://www.w3.org/2004/02/skos/core#inScheme"/>
                        <owl:hasValue rdf:resource="http://vocab.linkeddata.es/datosabiertos/kos/edint/VehiclePropulsionType"/>
                    </owl:Restriction>
                </owl:intersectionOf>
            </owl:Class>
        </rdfs:range>
        <rdfs:comment xml:lang="en">Propulsion type of a vehicle. The range is a SKOS concept that belongs to a controlled list of permit types (e.g., Diesel, Petrol, Electrical, etc.).</rdfs:comment>
        <rdfs:comment xml:lang="es">Tipo de propulsión de un vehículo. Los valores son conceptos SKOS que pertenecen a una lista controlada de tipos de autorización (por ejemplo, diésel, gasolina, eléctrico, etc.)</rdfs:comment>
        <rdfs:label xml:lang="en">propulsion type</rdfs:label>
        <rdfs:label xml:lang="es">tipo de propulsión</rdfs:label>
    </owl:ObjectProperty>
    


    <!-- http://vocab.linkeddata.es/datosabiertos/def/transporte/censovehiculos#registeredOwner -->


    <owl:ObjectProperty rdf:about="http://vocab.linkeddata.es/datosabiertos/def/transporte/censovehiculos#registeredOwner">
        <rdfs:domain rdf:resource="http://vocab.linkeddata.es/datosabiertos/def/transporte/censovehiculos#Vehicle"/>
        <rdfs:range rdf:resource="http://vocab.linkeddata.es/datosabiertos/def/transporte/censovehiculos#Owner"/>
        <rdfs:comment xml:lang="es">Identifica al titular (persona u organización) del vehículo</rdfs:comment>
        <rdfs:comment xml:lang="en">It identifies the person or organisation who owns the vehicle</rdfs:comment>
        <rdfs:comment xml:lang="en">registered owner</rdfs:comment>
        <rdfs:label xml:lang="es">titular registrado</rdfs:label>
    </owl:ObjectProperty>
    


    <!-- http://vocab.linkeddata.es/datosabiertos/def/transporte/censovehiculos#vehicleType -->


    <owl:ObjectProperty rdf:about="http://vocab.linkeddata.es/datosabiertos/def/transporte/censovehiculos#vehicleType">
        <rdfs:domain rdf:resource="http://vocab.linkeddata.es/datosabiertos/def/transporte/censovehiculos#Vehicle"/>
        <rdfs:range>
            <owl:Class>
                <owl:intersectionOf rdf:parseType="Collection">
                    <rdf:Description rdf:about="http://www.w3.org/2004/02/skos/core#Concept"/>
                    <owl:Restriction>
                        <owl:onProperty rdf:resource="http://www.w3.org/2004/02/skos/core#inScheme"/>
                        <owl:hasValue rdf:resource="http://vocab.linkeddata.es/datosabiertos/kos/edint/VehicleType"/>
                    </owl:Restriction>
                </owl:intersectionOf>
            </owl:Class>
        </rdfs:range>
        <rdfs:comment xml:lang="es">Tipo de vehículo. Los valores son conceptos SKOS que pertenecen a una lista controlada de tipos de autorización (por ejemplo, turismo, furgoneta, caravana, etc.)</rdfs:comment>
        <rdfs:comment xml:lang="en">Type of vehicle. The range is a SKOS concept that belongs to a controlled list of permit types (e.g., van, truck, caravan, etc.).</rdfs:comment>
        <rdfs:label xml:lang="es">tipo de vehículo</rdfs:label>
        <rdfs:label xml:lang="en">vehicle type</rdfs:label>
    </owl:ObjectProperty>
    


    <!-- http://www.w3.org/2004/02/skos/core#inScheme -->


    <owl:ObjectProperty rdf:about="http://www.w3.org/2004/02/skos/core#inScheme"/>
    


    <!-- 
    ///////////////////////////////////////////////////////////////////////////////////////
    //
    // Classes
    //
    ///////////////////////////////////////////////////////////////////////////////////////
     -->


    


    <!-- http://vocab.ciudadesabiertas.es/def/transporte/trafico#Tramo -->


    <owl:Class rdf:about="http://vocab.ciudadesabiertas.es/def/transporte/trafico#Tramo"/>
    


    <!-- http://vocab.linkeddata.es/datosabiertos/def/commons/zone#TrafficControlledZone -->


    <owl:Class rdf:about="http://vocab.linkeddata.es/datosabiertos/def/commons/zone#TrafficControlledZone"/>
    


    <!-- http://vocab.linkeddata.es/datosabiertos/def/transporte/censovehiculos#Owner -->


    <owl:Class rdf:about="http://vocab.linkeddata.es/datosabiertos/def/transporte/censovehiculos#Owner">
        <rdfs:subClassOf rdf:resource="https://schema.org/Organization"/>
        <rdfs:subClassOf rdf:resource="https://schema.org/Person"/>
        <rdfs:subClassOf>
            <owl:Class>
                <owl:unionOf rdf:parseType="Collection">
                    <rdf:Description rdf:about="https://schema.org/Organization"/>
                    <rdf:Description rdf:about="https://schema.org/Person"/>
                </owl:unionOf>
            </owl:Class>
        </rdfs:subClassOf>
        <rdfs:comment xml:lang="en">Owner</rdfs:comment>
        <rdfs:comment xml:lang="en">Person or organisation that is registered as the owner of a vehicle or of a vehicle permit</rdfs:comment>
        <rdfs:comment xml:lang="es">Persona u organización que está registrada como titular de un vehículo o como titular de una autorización para un vehículo</rdfs:comment>
        <rdfs:label xml:lang="es">Titular</rdfs:label>
    </owl:Class>
    


    <!-- http://vocab.linkeddata.es/datosabiertos/def/transporte/censovehiculos#Permit -->


    <owl:Class rdf:about="http://vocab.linkeddata.es/datosabiertos/def/transporte/censovehiculos#Permit">
        <rdfs:comment xml:lang="en">Official permit, usually issued by the city council or the traffic authority, that allows a particular vehicle to access, drive through, or park in an area where entry is restricted or regulated</rdfs:comment>
        <rdfs:comment xml:lang="es">Permiso oficial, emitido normalmente por el ayuntamiento o la autoridad de tráfico, que habilita a un vehículo concreto a acceder, circular o estacionar en un área donde el acceso está restringido o regulado</rdfs:comment>
        <rdfs:comment xml:lang="en">Permit</rdfs:comment>
        <rdfs:label xml:lang="es">Autorización</rdfs:label>
    </owl:Class>
    


    <!-- http://vocab.linkeddata.es/datosabiertos/def/transporte/censovehiculos#Vehicle -->


    <owl:Class rdf:about="http://vocab.linkeddata.es/datosabiertos/def/transporte/censovehiculos#Vehicle">
        <rdfs:subClassOf rdf:resource="https://saref.etsi.org/saref4auto/Vehicle/Vehicle"/>
        <rdfs:comment xml:lang="es">Dispositivo de transporte autopropulsado, junto con cualquier accesorio, por ejemplo remolques, que es un usuario legal de la red de transporte (Fuente: ISO/TS 19091:2019(en))</rdfs:comment>
        <rdfs:comment xml:lang="en">Self-propelled transport device, along with any attachments, e.g. trailers, that is a legal user of the transportation network (Source: ISO/TS 19091:2019(en)).</rdfs:comment>
        <rdfs:label xml:lang="en">Vehicle</rdfs:label>
        <rdfs:label xml:lang="es">Vehículo</rdfs:label>
    </owl:Class>
    


    <!-- http://www.w3.org/2004/02/skos/core#Concept -->


    <owl:Class rdf:about="http://www.w3.org/2004/02/skos/core#Concept"/>
    


    <!-- http://www.w3.org/2004/02/skos/core#ConceptScheme -->


    <owl:Class rdf:about="http://www.w3.org/2004/02/skos/core#ConceptScheme"/>
    


    <!-- https://saref.etsi.org/saref4auto/Vehicle/Vehicle -->


    <owl:Class rdf:about="https://saref.etsi.org/saref4auto/Vehicle/Vehicle"/>
    


    <!-- https://schema.org/Organization -->


    <owl:Class rdf:about="https://schema.org/Organization"/>
    


    <!-- https://schema.org/Person -->


    <owl:Class rdf:about="https://schema.org/Person"/>
    


    <!-- 
    ///////////////////////////////////////////////////////////////////////////////////////
    //
    // Individuals
    //
    ///////////////////////////////////////////////////////////////////////////////////////
     -->


    


    <!-- http://vocab.linkeddata.es/datosabiertos/kos/edint/VehicleEnvironmentalBadge -->


    <owl:NamedIndividual rdf:about="http://vocab.linkeddata.es/datosabiertos/kos/edint/VehicleEnvironmentalBadge">
        <rdf:type rdf:resource="http://www.w3.org/2004/02/skos/core#ConceptScheme"/>
    </owl:NamedIndividual>
    


    <!-- http://vocab.linkeddata.es/datosabiertos/kos/edint/VehiclePermitPeriodicity -->


    <owl:NamedIndividual rdf:about="http://vocab.linkeddata.es/datosabiertos/kos/edint/VehiclePermitPeriodicity">
        <rdf:type rdf:resource="http://www.w3.org/2004/02/skos/core#ConceptScheme"/>
    </owl:NamedIndividual>
    


    <!-- http://vocab.linkeddata.es/datosabiertos/kos/edint/VehiclePermitStatus -->


    <owl:NamedIndividual rdf:about="http://vocab.linkeddata.es/datosabiertos/kos/edint/VehiclePermitStatus">
        <rdf:type rdf:resource="http://www.w3.org/2004/02/skos/core#ConceptScheme"/>
    </owl:NamedIndividual>
    


    <!-- http://vocab.linkeddata.es/datosabiertos/kos/edint/VehiclePermitType -->


    <owl:NamedIndividual rdf:about="http://vocab.linkeddata.es/datosabiertos/kos/edint/VehiclePermitType">
        <rdf:type rdf:resource="http://www.w3.org/2004/02/skos/core#ConceptScheme"/>
    </owl:NamedIndividual>
    


    <!-- http://vocab.linkeddata.es/datosabiertos/kos/edint/VehiclePropulsionType -->


    <owl:NamedIndividual rdf:about="http://vocab.linkeddata.es/datosabiertos/kos/edint/VehiclePropulsionType">
        <rdf:type rdf:resource="http://www.w3.org/2004/02/skos/core#ConceptScheme"/>
    </owl:NamedIndividual>
    


    <!-- http://vocab.linkeddata.es/datosabiertos/kos/edint/VehicleType -->


    <owl:NamedIndividual rdf:about="http://vocab.linkeddata.es/datosabiertos/kos/edint/VehicleType">
        <rdf:type rdf:resource="http://www.w3.org/2004/02/skos/core#ConceptScheme"/>
    </owl:NamedIndividual>
    


    <!-- http://vocab.linkeddata.es/datosabiertos/kos/femp-base/registro-vehiculo#DistintivosAmbientales -->


    <owl:NamedIndividual rdf:about="http://vocab.linkeddata.es/datosabiertos/kos/femp-base/registro-vehiculo#DistintivosAmbientales"/>
    


    <!-- http://vocab.linkeddata.es/datosabiertos/kos/femp-base/registro-vehiculo#EstadosDeAutorización -->


    <owl:NamedIndividual rdf:about="http://vocab.linkeddata.es/datosabiertos/kos/femp-base/registro-vehiculo#EstadosDeAutorización"/>
    


    <!-- http://vocab.linkeddata.es/datosabiertos/kos/femp-base/registro-vehiculo#PeriodicidadAutorización -->


    <owl:NamedIndividual rdf:about="http://vocab.linkeddata.es/datosabiertos/kos/femp-base/registro-vehiculo#PeriodicidadAutorización"/>
    


    <!-- http://vocab.linkeddata.es/datosabiertos/kos/femp-base/registro-vehiculo#tipologiasPropulsión -->


    <owl:NamedIndividual rdf:about="http://vocab.linkeddata.es/datosabiertos/kos/femp-base/registro-vehiculo#tipologiasPropulsión"/>
    


    <!-- http://vocab.linkeddata.es/datosabiertos/kos/femp-base/registro-vehiculo#tipologiasVehiculo -->


    <owl:NamedIndividual rdf:about="http://vocab.linkeddata.es/datosabiertos/kos/femp-base/registro-vehiculo#tipologiasVehiculo"/>
    


    <!-- http://vocab.linkeddata.es/datosabiertos/kos/femp-base/registro-vehiculo#tiposDeAutorización -->


    <owl:NamedIndividual rdf:about="http://vocab.linkeddata.es/datosabiertos/kos/femp-base/registro-vehiculo#tiposDeAutorización"/>
</rdf:RDF>



<!-- Generated by the OWL API (version 5.1.18) https://github.com/owlcs/owlapi/ -->


